\section{Задание 6}
\[ I = \int \frac{2 x+3}{\sqrt{x^2+1} \left(x^2-2 x+1\right)} \, dx \]
Используем подстановку Эйлера:
\[ \sqrt{x^2+1} = x + t \]
\[ x = \frac{1-t^2}{2t} \]
\[ dx = -\frac{1+t^2}{2t^2} \, dt \]

\begin{multline*}
    I = \int  \frac{8 t \left(t^2-3 t-1\right)}
    {\left(t+\frac{1}{t}\right) \left(t^2+2 t-1\right)^2} \cdot
    \frac{1 + t^2}{2t^2} \, dt = 
    \int \frac{4 t \left(t^2-1\right) \left(t^2-3 t-1\right)}{\left(t^2+1\right)
    \left(t^2+2 t-1\right)^2} \, dt = \\ = \frac{at + b}{t^2+2t-1} + 
    \int \frac{ct^3 + dt^2 + et+f}{(t^2+2t-1)(1+t^2)} \, dt
\end{multline*}

\[ a = 11, b = -\frac{11}{2},c = 4,d= -9,e= 7,f= 0\]

\[
    I = \frac{11 (2 t-1)}{2 \left(t^2+2 t-1\right)} + \int \frac{4 t^3-9 t^2+7
    t}{\left(t^2+1\right) \left(t^2+2 t-1\right)} \, dt =
    \frac{11 (2 t-1)}{2 \left(t^2+2 t-1\right)} + I_1
\]

\begin{multline*}
    I_1 = \int \frac{4 t^3-9 t^2+7 t}{\left(t^2+1\right) \left(t^2+2 t-1\right)}
    \, dt = \int \frac{4t^3-9t^2+7t}{\left(t-\sqrt{2}+1\right)
    \left(t+\sqrt{2}+1\right)(t^2+1)} = \\
    = -\int \frac{3 (2 t+1)}{2 \left(t^2+1\right)} \, dt + \int \frac{17+14 \sqrt{2}}{4 \sqrt{2}
    \left(t+\sqrt{2}+1\right)} \, dt + \int \frac{17-14 \sqrt{2}}{4 \sqrt{2}
    \left(-t+\sqrt{2}-1\right)} \, dt \\ = \\ -\frac{3}{2} \ln
    \left(t^2+1\right)+\frac{1}{8} \left(28+17 \sqrt{2}\right) \ln
    \left(t+\sqrt{2}+1\right)+\frac{1}{8} \left(28-17 \sqrt{2}\right) \ln
    \left(8 t-8 \sqrt{2}+8\right)-\frac{3}{2}  \arctg t + C
\end{multline*}

\begin{multline*}
    I = \frac{11 (2 t-1)}{2 \left(t^2+2 t-1\right)} + -\frac{3}{2} \ln
    \left(t^2+1\right)+\frac{1}{8} \left(28+17 \sqrt{2}\right) \ln
    \left(t+\sqrt{2}+1\right)+ \\ +\frac{1}{8} \left(28-17 \sqrt{2}\right) \ln
\left(8 t-8 \sqrt{2}+8\right)-\frac{3}{2}  \arctg t + C,
\end{multline*}
где $ t = \sqrt{x^2+1} - x $.

